theories/wasm_parray.v
@@ -1,0 +1,167 @@
+(** A repackaged version of the persistent array interface in Rocq
+ *)
+
+From mathcomp Require Import ssreflect ssrbool eqtype seq ssrnat.
+From Coq Require Import ZArith Lia.
+From Wasm Require Export memory.
+
+Set Implicit Arguments.
+Unset Strict Implicit.
+Unset Printing Implicit Defensive.
+
+Open Scope N_scope.
+
+Global Parameter wasm_parrayof: Type -> Type.
+
+(* Persistent array, but removing some functions and relaxing the max_length
+   to 2^32-1. Also adding a different method of creating an array for
+   growing vectors.
+ *)
+Class Array := {
+    arr_make: forall A, N -> A -> wasm_parrayof A;
+    (* The same as make but initialises its prefix with values from
+   the prefix of another array.
+   Does not overflow if the length exceeds the make length.
+   This is used in the vector_grow function. *)
+    arr_make_copy: forall A, N -> A -> wasm_parrayof A -> N -> wasm_parrayof A;
+    arr_get : forall A, wasm_parrayof A -> N -> A;
+    arr_default : forall A, wasm_parrayof A -> A;
+    arr_set : forall A, wasm_parrayof A -> N -> A -> wasm_parrayof A;
+    (* Takes the length and the generator for the block *)
+    arr_set_gen : forall A, wasm_parrayof A -> N -> N -> (N -> A) -> wasm_parrayof A;
+    arr_length : forall A, wasm_parrayof A -> N;
+    arr_copy : forall A, wasm_parrayof A -> wasm_parrayof A;
+  }.
+
+Notation " t .[ i ] " := (arr_get t i) (at level 5).
+Notation " t .[ i <- a ] " := (arr_set t i a) (at level 5).
+
+(* Can't seem to assemble the type in OCaml since the type signature is not available *)
+
+Section Array_instance.
+
+  Parameter ocaml_arr_make: forall A, N -> A -> wasm_parrayof A.
+  (* The same as make but initialises its prefix with values from
+   the prefix of another Parameter ocaml_array.
+   Does not overflow if the length exceeds the make length.
+   This is used in the vector_grow function. *)
+  Parameter ocaml_arr_make_copy: forall A, N -> A -> wasm_parrayof A -> N -> wasm_parrayof A.
+  Parameter ocaml_arr_get : forall A, wasm_parrayof A -> N -> A.
+  Parameter ocaml_arr_default : forall A, wasm_parrayof A -> A.
+  Parameter ocaml_arr_set : forall A, wasm_parrayof A -> N -> A -> wasm_parrayof A.
+  (* Takes the length and the generator for the block *)
+  Parameter ocaml_arr_set_gen : forall A, wasm_parrayof A -> N -> N -> (N -> A) -> wasm_parrayof A.
+  Parameter ocaml_arr_length : forall A, wasm_parrayof A -> N.
+  Parameter ocaml_arr_copy : forall A, wasm_parrayof A -> wasm_parrayof A.
+
+  (* Putting the instance opaque so we don't unfold to the extraction primitives *)
+  Global Instance wasm_array_inst : Array.
+  Proof.
+    by refine {|
+      arr_make := ocaml_arr_make;
+      arr_make_copy := ocaml_arr_make_copy;
+      arr_get := ocaml_arr_get;
+      arr_default := ocaml_arr_default;
+      arr_set := ocaml_arr_set;
+      arr_set_gen := ocaml_arr_set_gen;
+      arr_length := ocaml_arr_length;
+      arr_copy := ocaml_arr_copy;
+      |}.
+  Qed.
+  
+End Array_instance.
+
+Definition max_arr_length : N := byte_limit.
+
+Section Array_axioms.
+
+Context {A: Type}.
+
+Local Definition array := wasm_parrayof A.
+
+Parameter get_out_of_bounds :
+  forall (t : array) (i : N),
+    N.ltb i (arr_length t) = false -> t.[i] = arr_default t.
+Parameter get_set_same :
+  forall (t : array) (i : N) (a : A),
+    N.ltb i (arr_length t) = true -> t.[i<-a].[i] = a.
+Parameter get_set_other :
+  forall (t : array) (i j : N) (a : A),
+    i <> j -> t.[i<-a].[j] = t.[j].
+Parameter default_set :
+  forall (t : array) (i : N) (a : A),
+    arr_default t.[i<-a] = arr_default t.
+Parameter get_make :
+  forall (a : A) (size i : N),
+    (arr_make size a).[i] = a.
+Parameter get_make_copy:
+  forall (a: A) (size i: N) (t: array) (initlen: N),
+    N.ltb i size ->
+    N.leb initlen (arr_length t) ->
+    N.ltb i (arr_length t) ->
+    (arr_make_copy size a t initlen).[i] = t.[i].
+Parameter get_make_copy_default:
+  forall (a: A) (size i: N) (t: array) (initlen: N),
+    N.ltb i size ->
+    N.leb initlen (arr_length t) ->
+    N.leb initlen i ->
+    (arr_make_copy size a t initlen).[i] = a.
+Parameter leb_length :
+  forall (t : array),
+    N.leb (arr_length t) max_arr_length = true.
+Parameter length_make :
+  forall (size : N) (a : A),
+    arr_length (arr_make size a) =
+      N.min size max_arr_length.
+Parameter length_make_copy :
+  forall (size : N) (a : A) (t: array) (initlen: N),
+    arr_length (arr_make_copy size a t initlen) =
+      N.min size max_arr_length.
+Parameter length_set :
+  forall (t : array) (i : N) (a : A),
+    arr_length t.[i<-a] = arr_length t.
+
+(* Some added axioms for set_gen *)
+Parameter length_set_gen :
+  forall (t : array) (i : N) (len: N) (gen: N -> A),
+    arr_length (arr_set_gen t i len gen) = arr_length t.
+
+Parameter arr_set_gen_lookup:
+  forall n len gen (t: array) i,
+    N.ltb i len ->
+    arr_get (arr_set_gen t n len gen) (N.add n i) = (gen i).
+
+Parameter arr_set_gen_lt:
+  forall n len gen (t: array) i,
+    N.ltb i n ->
+    arr_get (arr_set_gen t n len gen) i = arr_get t i.
+
+Parameter arr_set_gen_ge:
+  forall n len gen (t: array) i,
+    N.leb (N.add n len) i ->
+    arr_get (arr_set_gen t n len gen) i = arr_get t i.
+                                         
+Parameter get_copy :
+  forall (t : array) (i : N),
+    (arr_copy t).[i] = t.[i].
+Parameter length_copy :
+  forall (t : array), arr_length (arr_copy t) = arr_length t.
+Parameter array_ext :
+  forall (t1 t2 : array),
+    arr_length t1 = arr_length t2 ->
+    (forall i : N,
+        N.ltb i (arr_length t1) = true -> t1.[i] = t2.[i]) ->
+    arr_default t1 = arr_default t2 -> t1 = t2.
+Parameter default_copy :
+  forall (t : array), arr_default (arr_copy t) = arr_default t.
+Parameter default_make :
+  forall (a : A) (size : N),
+    arr_default (arr_make size a) = a.
+Parameter get_set_same_default :
+  forall (t : array) (i : N),
+    t.[i<-arr_default t].[i] = arr_default t.
+Parameter get_not_default_lt :
+  forall (t : array) (x : N),
+    t.[x] <> arr_default t -> N.ltb x (arr_length t) = true.
+
+End Array_axioms.
